Equiv.v
@@ -2,7 +2,7 @@ Require Import Coq.Program.Equality.
 Require Import List ZArith.
 Require Import Arith.
 Require Import Psatz.
-Require Import Omega.
+Require Import Lia.
 Import ListNotations.
 Open Scope nat_scope.
 Close Scope Z_scope.
@@ -11,13 +11,12 @@ Open Scope string_scope.
 Require Import While Tactics.
 Require Import WhileSmallStep WhileBigStep.
 
-
 Lemma star_seq:
   forall s1 env1 env2,
-    star s1 env1 Skip env2 ->
-    forall s2 s3 env3,
-      star s2 env2 s3 env3 ->
-      star (Seq s1 s2) env1 s3 env3.
+  star s1 env1 Skip env2
+  -> forall s2 s3 env3,
+  star s2 env2 s3 env3
+  -> star (Seq s1 s2) env1 s3 env3.
 Proof.
   intros s1 env1 env2 Hstar.
   dependent induction Hstar; simpl; intros.
@@ -25,9 +24,7 @@ Admitted.
 
 
 Theorem bigstep_star:
-  forall i env env',
-    bigstep env i env' ->
-    star i env Skip env'.
+  forall i env env', bigstep env i env' -> star i env Skip env'.
 Proof.
 Admitted.
 
@@ -41,9 +38,7 @@ Proof.
 Admitted.
 
 Theorem star_bigstep:
-  forall i env env',
-    star i env Skip env' ->
-    bigstep env i env'.
+  forall i env env', star i env Skip env' -> bigstep env i env'.
 Proof.
 Admitted.
 
