Interp.v
@@ -2,7 +2,7 @@ Require Import Coq.Program.Equality.
 Require Import List ZArith.
 Require Import Arith.
 Require Import Psatz.
-Require Import Omega.
+Require Import Lia.
 Import ListNotations.
 Open Scope nat_scope.
 Close Scope Z_scope.
@@ -16,44 +16,42 @@ Fixpoint exec_prog (fuel: nat) (env: state) (i: stmt) : option state :=
 None.
 
 Definition p1 :=
-  Seq (Assign "x" (Const 10%Z))
-      (Seq (Assign "sum" (Const 0%Z))
-           (While (Not (Eq (Var "x") (Const 0%Z)))
-                  (fun _ => True)
-                  (Seq
-                     (Assign "sum" (Add (Var "sum") (Var "x")))
-                     (Assign "x" (Sub (Var "x") (Const 1%Z)))
-                  )
-           )
-      ).
+  Seq
+    (Assign "x" (Const 10%Z))
+    (Seq
+      (Assign "sum" (Const 0%Z))
+      (While
+        (Not (Eq (Var "x") (Const 0%Z)))
+        (fun _ => True)
+        (Seq
+          (Assign "sum" (Add (Var "sum") (Var "x")))
+          (Assign "x" (Sub (Var "x") (Const 1%Z)))
+        )
+      )
+    ).
 
 (* Le calcul suivant devrait retourner [Some 55]. *)
 Compute
   option_map (fun env => env "sum")
   (exec_prog 30 (fun _ => 0%Z) p1).
 
-
 Theorem exec_prog_bigstep:
-  forall fuel s i s',
-    exec_prog fuel s i = Some s' ->
-    bigstep s i s'.
+  forall fuel s i s', exec_prog fuel s i = Some s' -> bigstep s i s'.
 Proof.
 Admitted.
 
 Lemma exec_prog_more_fuel:
   forall f s i s',
-    exec_prog f s i = Some s' ->
-    forall f',
-      f' >= f ->
-      exec_prog f' s i = Some s'.
+  exec_prog f s i = Some s'
+  -> forall f', f' >= f
+  -> exec_prog f' s i = Some s'.
 Proof.
 Admitted.
 
 Theorem bigstep_exec_prog:
   forall s i s',
-    bigstep s i s' ->
-    exists fuel,
-      exec_prog fuel s i = Some s'.
+  bigstep s i s'
+  -> exists fuel, exec_prog fuel s i = Some s'.
 Proof.
 Admitted.
 
