Tactics.v
@@ -1,20 +1,17 @@
 Ltac inv H := inversion H; try subst; clear H.
 
-
 Ltac trim H :=
   match type of H with
-    ?A -> ?B => let x := fresh in
-                assert (x: A); [clear H| specialize (H x); clear x]
+  | ?A -> ?B =>
+    let x := fresh in
+    assert (x: A); [clear H| specialize (H x); clear x]
   end.
 
 Require Import Arith ZArith Lia.
 
 Definition Zfact n := Z.of_nat (fact (Z.to_nat n)).
 
-Lemma fact_S:
-  (forall n : nat,
-    n <> 0 ->
-    fact n = n * fact (n - 1))%nat.
+Lemma fact_S: (forall n : nat, n <> 0 -> fact n = n * fact (n - 1))%nat.
 Proof.
   destruct n; simpl; auto. congruence.
   rewrite ! Nat.sub_0_r.  auto.
@@ -22,9 +19,7 @@ Qed.
 
 Open Scope Z_scope.
 
-Lemma Zfact_pos:
-  forall z, 0 < z ->
-            Zfact z = z * Zfact (z - 1).
+Lemma Zfact_pos: forall z, 0 < z -> Zfact z = z * Zfact (z - 1).
 Proof.
   unfold Zfact. intros.
   rewrite (fact_S (Z.to_nat z)). 2: lia.
@@ -33,30 +28,25 @@ Proof.
   rewrite Z2Nat.id. 2: lia. reflexivity.
 Qed.
 
-Lemma Zfact_neg:
-  forall z,
-    z <= 0 ->
-    Zfact z = 1.
+Lemma Zfact_neg: forall z, z <= 0 -> Zfact z = 1.
 Proof.
   unfold Zfact; intros.
   unfold Z.to_nat.
   destruct z; simpl; auto. lia.
 Qed.
 
-
 Fixpoint fib n :=
   (match n with
   | O => 1%nat
-  | S n' => match n' with
-            | O => 1
-            | S n'' => fib n' + fib n''
-            end
+  | S n' =>
+    match n' with
+    | O => 1
+    | S n'' => fib n' + fib n''
+    end
   end)%nat.
 
 Lemma fib_eqn (n: nat) : (n > 0 -> fib n + fib (Nat.pred n) = fib (1 + n))%nat.
-Proof.
-  induction n; simpl; intros; eauto. lia.
-Qed.
+Proof. induction n; simpl; intros; eauto. lia. Qed.
 
 Definition Zfib n := Z.of_nat (fib (Z.to_nat n)).
 
